strengthen a_wf_wl def

proof/iu_system/uni/def_ott.v
@@ -63,11 +63,6 @@ Inductive abind : Set :=
  | abind_typ (A:typ)
  | abind_bound (A1:typ) (B1:typ).
 
-Inductive dvalue : Set := 
- | dvalue_unit : dvalue
- | dvalue_abs (e:exp)
- | dvalue_tabs (body5:body).
-
 Inductive dworklist : Set := 
  | dworklist_empty : dworklist
  | dworklist_consvar (Ω:dworklist) (x:expvar) (db:dbind)
@@ -76,13 +71,18 @@ Inductive dworklist : Set :=
 
 Definition aenv : Set := list (atom*abind).
 
+Inductive dvalue : Set := 
+ | dvalue_unit : dvalue
+ | dvalue_abs (e:exp)
+ | dvalue_tabs (body5:body).
+
+Definition denv : Set := list (atom*dbind).
+
 Inductive aworklist : Set := 
  | aworklist_empty : aworklist
  | aworklist_consvar (aW:aworklist) (x:expvar) (ab:abind)
  | aworklist_constvar (aW:aworklist) (X:typvar) (ab:abind)
  | aworklist_conswork (aW:aworklist) (w:work).
-
-Definition denv : Set := list (atom*dbind).
 
 (* EXPERIMENTAL *)
 (** auxiliary functions on the new list types *)
@@ -311,7 +311,11 @@ Fixpoint close_typ_wrt_typ_rec (k:nat) (A_5:var) (A__6:typ) {struct A__6}: typ :
   | (typ_intersection A1 A2) => typ_intersection (close_typ_wrt_typ_rec k A_5 A1) (close_typ_wrt_typ_rec k A_5 A2)
 end.
 
-Fixpoint close_exp_wrt_typ_rec (k:nat) (A_5:var) (e_5:exp) {struct e_5}: exp :=
+Fixpoint close_body_wrt_typ_rec (k:nat) (A5:var) (body5:body) : body :=
+  match body5 with
+  | (body_anno e A) => body_anno (close_exp_wrt_typ_rec k A5 e) (close_typ_wrt_typ_rec k A5 A)
+end
+with close_exp_wrt_typ_rec (k:nat) (A_5:var) (e_5:exp) {struct e_5}: exp :=
   match e_5 with
   | exp_unit => exp_unit 
   | (exp_var_b nat) => exp_var_b nat
@@ -321,10 +325,6 @@ Fixpoint close_exp_wrt_typ_rec (k:nat) (A_5:var) (e_5:exp) {struct e_5}: exp :=
   | (exp_tabs body5) => exp_tabs (close_body_wrt_typ_rec (S k) A_5 body5)
   | (exp_tapp e A) => exp_tapp (close_exp_wrt_typ_rec k A_5 e) (close_typ_wrt_typ_rec k A_5 A)
   | (exp_anno e A) => exp_anno (close_exp_wrt_typ_rec k A_5 e) (close_typ_wrt_typ_rec k A_5 A)
-end
-with close_body_wrt_typ_rec (k:nat) (A5:var) (body5:body) : body :=
-  match body5 with
-  | (body_anno e A) => body_anno (close_exp_wrt_typ_rec k A5 e) (close_typ_wrt_typ_rec k A5 A)
 end.
 
 Fixpoint close_exp_wrt_exp_rec (k:nat) (e_5:var) (e__6:exp) {struct e__6}: exp :=
@@ -423,6 +423,29 @@ Fixpoint close_aworklist_wrt_typ_rec (k:nat) (A5:var) (aW_5:aworklist) {struct a
   | (aworklist_conswork aW w) => aworklist_conswork (close_aworklist_wrt_typ_rec k A5 aW) (close_work_wrt_typ_rec k A5 w)
 end.
 
+Fixpoint close_dworklist_wrt_exp_rec (k:nat) (e5:var) (Ω5:dworklist) {struct Ω5}: dworklist :=
+  match Ω5 with
+  | dworklist_empty => dworklist_empty 
+  | (dworklist_consvar Ω x db) => dworklist_consvar (close_dworklist_wrt_exp_rec k e5 Ω) x db
+  | (dworklist_constvar Ω X db) => dworklist_constvar (close_dworklist_wrt_exp_rec k e5 Ω) X db
+  | (dworklist_conswork Ω w) => dworklist_conswork (close_dworklist_wrt_exp_rec k e5 Ω) (close_work_wrt_exp_rec k e5 w)
+end.
+
+Fixpoint close_dworklist_wrt_typ_rec (k:nat) (A5:var) (Ω5:dworklist) {struct Ω5}: dworklist :=
+  match Ω5 with
+  | dworklist_empty => dworklist_empty 
+  | (dworklist_consvar Ω x db) => dworklist_consvar (close_dworklist_wrt_typ_rec k A5 Ω) x (close_dbind_wrt_typ_rec k A5 db)
+  | (dworklist_constvar Ω X db) => dworklist_constvar (close_dworklist_wrt_typ_rec k A5 Ω) X (close_dbind_wrt_typ_rec k A5 db)
+  | (dworklist_conswork Ω w) => dworklist_conswork (close_dworklist_wrt_typ_rec k A5 Ω) (close_work_wrt_typ_rec k A5 w)
+end.
+
+Definition close_dvalue_wrt_typ_rec (k:nat) (A5:var) (v5:dvalue) : dvalue :=
+  match v5 with
+  | dvalue_unit => dvalue_unit 
+  | (dvalue_abs e) => dvalue_abs (close_exp_wrt_typ_rec k A5 e)
+  | (dvalue_tabs body5) => dvalue_tabs (close_body_wrt_typ_rec (S k) A5 body5)
+end.
+
 Definition close_dvalue_wrt_exp_rec (k:nat) (e5:var) (v5:dvalue) : dvalue :=
   match v5 with
   | dvalue_unit => dvalue_unit 
@@ -438,62 +461,39 @@ Fixpoint close_aworklist_wrt_exp_rec (k:nat) (e5:var) (aW_5:aworklist) {struct a
   | (aworklist_conswork aW w) => aworklist_conswork (close_aworklist_wrt_exp_rec k e5 aW) (close_work_wrt_exp_rec k e5 w)
 end.
 
-Fixpoint close_dworklist_wrt_exp_rec (k:nat) (e5:var) (Ω5:dworklist) {struct Ω5}: dworklist :=
-  match Ω5 with
-  | dworklist_empty => dworklist_empty 
-  | (dworklist_consvar Ω x db) => dworklist_consvar (close_dworklist_wrt_exp_rec k e5 Ω) x db
-  | (dworklist_constvar Ω X db) => dworklist_constvar (close_dworklist_wrt_exp_rec k e5 Ω) X db
-  | (dworklist_conswork Ω w) => dworklist_conswork (close_dworklist_wrt_exp_rec k e5 Ω) (close_work_wrt_exp_rec k e5 w)
-end.
-
-Definition close_dvalue_wrt_typ_rec (k:nat) (A5:var) (v5:dvalue) : dvalue :=
-  match v5 with
-  | dvalue_unit => dvalue_unit 
-  | (dvalue_abs e) => dvalue_abs (close_exp_wrt_typ_rec k A5 e)
-  | (dvalue_tabs body5) => dvalue_tabs (close_body_wrt_typ_rec (S k) A5 body5)
-end.
-
-Fixpoint close_dworklist_wrt_typ_rec (k:nat) (A5:var) (Ω5:dworklist) {struct Ω5}: dworklist :=
-  match Ω5 with
-  | dworklist_empty => dworklist_empty 
-  | (dworklist_consvar Ω x db) => dworklist_consvar (close_dworklist_wrt_typ_rec k A5 Ω) x (close_dbind_wrt_typ_rec k A5 db)
-  | (dworklist_constvar Ω X db) => dworklist_constvar (close_dworklist_wrt_typ_rec k A5 Ω) X (close_dbind_wrt_typ_rec k A5 db)
-  | (dworklist_conswork Ω w) => dworklist_conswork (close_dworklist_wrt_typ_rec k A5 Ω) (close_work_wrt_typ_rec k A5 w)
-end.
-
-Definition close_aworklist_wrt_typ aW_5 A5 := close_aworklist_wrt_typ_rec 0 aW_5 A5.
-
-Definition close_dvalue_wrt_exp v5 e5 := close_dvalue_wrt_exp_rec 0 v5 e5.
-
-Definition close_abind_wrt_typ ab5 A_5 := close_abind_wrt_typ_rec 0 ab5 A_5.
-
 Definition close_work_wrt_typ w5 A_5 := close_work_wrt_typ_rec 0 w5 A_5.
-
-Definition close_dbind_wrt_typ db5 A5 := close_dbind_wrt_typ_rec 0 db5 A5.
-
-Definition close_aworklist_wrt_exp aW_5 e5 := close_aworklist_wrt_exp_rec 0 aW_5 e5.
-
-Definition close_exp_wrt_exp e__6 e_5 := close_exp_wrt_exp_rec 0 e__6 e_5.
-
-Definition close_cont_wrt_typ c5 A_5 := close_cont_wrt_typ_rec 0 c5 A_5.
-
-Definition close_dworklist_wrt_exp Ω5 e5 := close_dworklist_wrt_exp_rec 0 Ω5 e5.
-
-Definition close_exp_wrt_typ e_5 A_5 := close_exp_wrt_typ_rec 0 e_5 A_5.
 
 Definition close_body_wrt_typ body5 A5 := close_body_wrt_typ_rec 0 body5 A5.
 
-Definition close_typ_wrt_typ A__6 A_5 := close_typ_wrt_typ_rec 0 A__6 A_5.
+Definition close_abind_wrt_typ ab5 A_5 := close_abind_wrt_typ_rec 0 ab5 A_5.
 
-Definition close_cont_wrt_exp c5 e5 := close_cont_wrt_exp_rec 0 c5 e5.
+Definition close_exp_wrt_typ e_5 A_5 := close_exp_wrt_typ_rec 0 e_5 A_5.
+
+Definition close_aworklist_wrt_typ aW_5 A5 := close_aworklist_wrt_typ_rec 0 aW_5 A5.
 
 Definition close_work_wrt_exp w5 e5 := close_work_wrt_exp_rec 0 w5 e5.
 
-Definition close_dvalue_wrt_typ v5 A5 := close_dvalue_wrt_typ_rec 0 v5 A5.
+Definition close_exp_wrt_exp e__6 e_5 := close_exp_wrt_exp_rec 0 e__6 e_5.
+
+Definition close_dworklist_wrt_exp Ω5 e5 := close_dworklist_wrt_exp_rec 0 Ω5 e5.
 
 Definition close_dworklist_wrt_typ Ω5 A5 := close_dworklist_wrt_typ_rec 0 Ω5 A5.
 
+Definition close_cont_wrt_typ c5 A_5 := close_cont_wrt_typ_rec 0 c5 A_5.
+
+Definition close_dbind_wrt_typ db5 A5 := close_dbind_wrt_typ_rec 0 db5 A5.
+
+Definition close_dvalue_wrt_typ v5 A5 := close_dvalue_wrt_typ_rec 0 v5 A5.
+
+Definition close_typ_wrt_typ A__6 A_5 := close_typ_wrt_typ_rec 0 A__6 A_5.
+
+Definition close_dvalue_wrt_exp v5 e5 := close_dvalue_wrt_exp_rec 0 v5 e5.
+
+Definition close_aworklist_wrt_exp aW_5 e5 := close_aworklist_wrt_exp_rec 0 aW_5 e5.
+
 Definition close_body_wrt_exp body5 e5 := close_body_wrt_exp_rec 0 body5 e5.
+
+Definition close_cont_wrt_exp c5 e5 := close_cont_wrt_exp_rec 0 c5 e5.
 
 (** terms are locally-closed pre-terms *)
 (** definitions *)
@@ -666,17 +666,6 @@ Inductive lc_abind : abind -> Prop :=    (* defn lc_abind *)
      (lc_typ B1) ->
      (lc_abind (abind_bound A1 B1)).
 
-(* defns LC_dvalue *)
-Inductive lc_dvalue : dvalue -> Prop :=    (* defn lc_dvalue *)
- | lc_dvalue_unit : 
-     (lc_dvalue dvalue_unit)
- | lc_dvalue_abs : forall (e:exp),
-      ( forall x , lc_exp  ( open_exp_wrt_exp e (exp_var_f x) )  )  ->
-     (lc_dvalue (dvalue_abs e))
- | lc_dvalue_tabs : forall (body5:body),
-      ( forall X , lc_body  ( open_body_wrt_typ body5 (typ_var_f X) )  )  ->
-     (lc_dvalue (dvalue_tabs body5)).
-
 (* defns LC_dworklist *)
 Inductive lc_dworklist : dworklist -> Prop :=    (* defn lc_dworklist *)
  | lc_dworklist_empty : 
@@ -693,6 +682,17 @@ Inductive lc_dworklist : dworklist -> Prop :=    (* defn lc_dworklist *)
      (lc_dworklist Ω) ->
      (lc_work w) ->
      (lc_dworklist (dworklist_conswork Ω w)).
+
+(* defns LC_dvalue *)
+Inductive lc_dvalue : dvalue -> Prop :=    (* defn lc_dvalue *)
+ | lc_dvalue_unit : 
+     (lc_dvalue dvalue_unit)
+ | lc_dvalue_abs : forall (e:exp),
+      ( forall x , lc_exp  ( open_exp_wrt_exp e (exp_var_f x) )  )  ->
+     (lc_dvalue (dvalue_abs e))
+ | lc_dvalue_tabs : forall (body5:body),
+      ( forall X , lc_body  ( open_body_wrt_typ body5 (typ_var_f X) )  )  ->
+     (lc_dvalue (dvalue_tabs body5)).
 
 (* defns LC_aworklist *)
 Inductive lc_aworklist : aworklist -> Prop :=    (* defn lc_aworklist *)
@@ -780,13 +780,6 @@ Fixpoint fvar_in_cont (c5:cont) : vars :=
   | (cont_sub A) => {}
 end.
 
-Definition ftvar_in_dbind (db5:dbind) : vars :=
-  match db5 with
-  | dbind_tvar_empty => {}
-  | dbind_stvar_empty => {}
-  | (dbind_typ A) => (ftvar_in_typ A)
-end.
-
 Definition ftvar_in_work (w5:work) : vars :=
   match w5 with
   | (work_infer e c) => (ftvar_in_exp e) \u (ftvar_in_cont c)
@@ -800,6 +793,14 @@ Definition ftvar_in_work (w5:work) : vars :=
   | (work_unioninftapp A1 A2 c) => (ftvar_in_typ A1) \u (ftvar_in_typ A2) \u (ftvar_in_cont c)
   | (work_unioninfabs A1 A2 c) => (ftvar_in_typ A1) \u (ftvar_in_typ A2) \u (ftvar_in_cont c)
   | (work_apply c A) => (ftvar_in_cont c) \u (ftvar_in_typ A)
+end.
+
+Definition ftvar_in_abind (ab5:abind) : vars :=
+  match ab5 with
+  | abind_tvar_empty => {}
+  | abind_stvar_empty => {}
+  | (abind_typ A) => (ftvar_in_typ A)
+  | (abind_bound A1 B1) => (ftvar_in_typ A1) \u (ftvar_in_typ B1)
 end.
 
 Definition fvar_in_work (w5:work) : vars :=
@@ -817,35 +818,11 @@ Definition fvar_in_work (w5:work) : vars :=
   | (work_apply c A) => (fvar_in_cont c)
 end.
 
-Definition ftvar_in_abind (ab5:abind) : vars :=
-  match ab5 with
-  | abind_tvar_empty => {}
-  | abind_stvar_empty => {}
-  | (abind_typ A) => (ftvar_in_typ A)
-  | (abind_bound A1 B1) => (ftvar_in_typ A1) \u (ftvar_in_typ B1)
-end.
-
-Fixpoint ftvar_in_dworklist (Ω5:dworklist) : vars :=
-  match Ω5 with
-  | dworklist_empty => {}
-  | (dworklist_consvar Ω x db) => (ftvar_in_dworklist Ω) \u (ftvar_in_dbind db)
-  | (dworklist_constvar Ω X db) => (ftvar_in_dworklist Ω) \u (ftvar_in_dbind db)
-  | (dworklist_conswork Ω w) => (ftvar_in_dworklist Ω) \u (ftvar_in_work w)
-end.
-
-Definition fvar_in_dvalue (v5:dvalue) : vars :=
-  match v5 with
-  | dvalue_unit => {}
-  | (dvalue_abs e) => (fvar_in_exp e)
-  | (dvalue_tabs body5) => (fvar_in_body body5)
-end.
-
-Fixpoint fvar_in_dworklist (Ω5:dworklist) : vars :=
-  match Ω5 with
-  | dworklist_empty => {}
-  | (dworklist_consvar Ω x db) => (fvar_in_dworklist Ω)
-  | (dworklist_constvar Ω X db) => (fvar_in_dworklist Ω)
-  | (dworklist_conswork Ω w) => (fvar_in_dworklist Ω) \u (fvar_in_work w)
+Definition ftvar_in_dbind (db5:dbind) : vars :=
+  match db5 with
+  | dbind_tvar_empty => {}
+  | dbind_stvar_empty => {}
+  | (dbind_typ A) => (ftvar_in_typ A)
 end.
 
 Fixpoint ftvar_in_aworklist (aW_5:aworklist) : vars :=
@@ -871,6 +848,29 @@ Definition ftvar_in_dvalue (v5:dvalue) : vars :=
   | (dvalue_tabs body5) => (ftvar_in_body body5)
 end.
 
+Fixpoint ftvar_in_dworklist (Ω5:dworklist) : vars :=
+  match Ω5 with
+  | dworklist_empty => {}
+  | (dworklist_consvar Ω x db) => (ftvar_in_dworklist Ω) \u (ftvar_in_dbind db)
+  | (dworklist_constvar Ω X db) => (ftvar_in_dworklist Ω) \u (ftvar_in_dbind db)
+  | (dworklist_conswork Ω w) => (ftvar_in_dworklist Ω) \u (ftvar_in_work w)
+end.
+
+Definition fvar_in_dvalue (v5:dvalue) : vars :=
+  match v5 with
+  | dvalue_unit => {}
+  | (dvalue_abs e) => (fvar_in_exp e)
+  | (dvalue_tabs body5) => (fvar_in_body body5)
+end.
+
+Fixpoint fvar_in_dworklist (Ω5:dworklist) : vars :=
+  match Ω5 with
+  | dworklist_empty => {}
+  | (dworklist_consvar Ω x db) => (fvar_in_dworklist Ω)
+  | (dworklist_constvar Ω X db) => (fvar_in_dworklist Ω)
+  | (dworklist_conswork Ω w) => (fvar_in_dworklist Ω) \u (fvar_in_work w)
+end.
+
 (** substitutions *)
 Fixpoint subst_tvar_in_typ (A_5:typ) (X5:typvar) (A__6:typ) {struct A__6} : typ :=
   match A__6 with
@@ -883,22 +883,6 @@ Fixpoint subst_tvar_in_typ (A_5:typ) (X5:typvar) (A__6:typ) {struct A__6} : typ 
   | (typ_all A) => typ_all (subst_tvar_in_typ A_5 X5 A)
   | (typ_union A1 A2) => typ_union (subst_tvar_in_typ A_5 X5 A1) (subst_tvar_in_typ A_5 X5 A2)
   | (typ_intersection A1 A2) => typ_intersection (subst_tvar_in_typ A_5 X5 A1) (subst_tvar_in_typ A_5 X5 A2)
-end.
-
-Fixpoint subst_var_in_exp (e_5:exp) (x5:expvar) (e__6:exp) {struct e__6} : exp :=
-  match e__6 with
-  | exp_unit => exp_unit 
-  | (exp_var_b nat) => exp_var_b nat
-  | (exp_var_f x) => (if eq_var x x5 then e_5 else (exp_var_f x))
-  | (exp_abs e) => exp_abs (subst_var_in_exp e_5 x5 e)
-  | (exp_app e1 e2) => exp_app (subst_var_in_exp e_5 x5 e1) (subst_var_in_exp e_5 x5 e2)
-  | (exp_tabs body5) => exp_tabs (subst_var_in_body e_5 x5 body5)
-  | (exp_tapp e A) => exp_tapp (subst_var_in_exp e_5 x5 e) A
-  | (exp_anno e A) => exp_anno (subst_var_in_exp e_5 x5 e) A
-end
-with subst_var_in_body (e5:exp) (x5:expvar) (body5:body) {struct body5} : body :=
-  match body5 with
-  | (body_anno e A) => body_anno (subst_var_in_exp e5 x5 e) A
 end.
 
 Fixpoint subst_tvar_in_exp (A_5:typ) (X5:typvar) (e_5:exp) {struct e_5} : exp :=
@@ -917,16 +901,20 @@ with subst_tvar_in_body (A5:typ) (X5:typvar) (body5:body) {struct body5} : body 
   | (body_anno e A) => body_anno (subst_tvar_in_exp A5 X5 e) (subst_tvar_in_typ A5 X5 A)
 end.
 
-Fixpoint subst_var_in_cont (e5:exp) (x5:expvar) (c5:cont) {struct c5} : cont :=
-  match c5 with
-  | (cont_infabs c) => cont_infabs (subst_var_in_cont e5 x5 c)
-  | (cont_infabsunion A1 c) => cont_infabsunion A1 (subst_var_in_cont e5 x5 c)
-  | (cont_infapp e c) => cont_infapp (subst_var_in_exp e5 x5 e) (subst_var_in_cont e5 x5 c)
-  | (cont_inftapp A c) => cont_inftapp A (subst_var_in_cont e5 x5 c)
-  | (cont_inftappunion A1 A2 c) => cont_inftappunion A1 A2 (subst_var_in_cont e5 x5 c)
-  | (cont_unioninftapp A2 c) => cont_unioninftapp A2 (subst_var_in_cont e5 x5 c)
-  | (cont_unioninfabs A2 c) => cont_unioninfabs A2 (subst_var_in_cont e5 x5 c)
-  | (cont_sub A) => cont_sub A
+Fixpoint subst_var_in_exp (e_5:exp) (x5:expvar) (e__6:exp) {struct e__6} : exp :=
+  match e__6 with
+  | exp_unit => exp_unit 
+  | (exp_var_b nat) => exp_var_b nat
+  | (exp_var_f x) => (if eq_var x x5 then e_5 else (exp_var_f x))
+  | (exp_abs e) => exp_abs (subst_var_in_exp e_5 x5 e)
+  | (exp_app e1 e2) => exp_app (subst_var_in_exp e_5 x5 e1) (subst_var_in_exp e_5 x5 e2)
+  | (exp_tabs body5) => exp_tabs (subst_var_in_body e_5 x5 body5)
+  | (exp_tapp e A) => exp_tapp (subst_var_in_exp e_5 x5 e) A
+  | (exp_anno e A) => exp_anno (subst_var_in_exp e_5 x5 e) A
+end
+with subst_var_in_body (e5:exp) (x5:expvar) (body5:body) {struct body5} : body :=
+  match body5 with
+  | (body_anno e A) => body_anno (subst_var_in_exp e5 x5 e) A
 end.
 
 Fixpoint subst_tvar_in_cont (A_5:typ) (X5:typvar) (c5:cont) {struct c5} : cont :=
@@ -939,6 +927,40 @@ Fixpoint subst_tvar_in_cont (A_5:typ) (X5:typvar) (c5:cont) {struct c5} : cont :
   | (cont_unioninftapp A2 c) => cont_unioninftapp (subst_tvar_in_typ A_5 X5 A2) (subst_tvar_in_cont A_5 X5 c)
   | (cont_unioninfabs A2 c) => cont_unioninfabs (subst_tvar_in_typ A_5 X5 A2) (subst_tvar_in_cont A_5 X5 c)
   | (cont_sub A) => cont_sub (subst_tvar_in_typ A_5 X5 A)
+end.
+
+Fixpoint subst_var_in_cont (e5:exp) (x5:expvar) (c5:cont) {struct c5} : cont :=
+  match c5 with
+  | (cont_infabs c) => cont_infabs (subst_var_in_cont e5 x5 c)
+  | (cont_infabsunion A1 c) => cont_infabsunion A1 (subst_var_in_cont e5 x5 c)
+  | (cont_infapp e c) => cont_infapp (subst_var_in_exp e5 x5 e) (subst_var_in_cont e5 x5 c)
+  | (cont_inftapp A c) => cont_inftapp A (subst_var_in_cont e5 x5 c)
+  | (cont_inftappunion A1 A2 c) => cont_inftappunion A1 A2 (subst_var_in_cont e5 x5 c)
+  | (cont_unioninftapp A2 c) => cont_unioninftapp A2 (subst_var_in_cont e5 x5 c)
+  | (cont_unioninfabs A2 c) => cont_unioninfabs A2 (subst_var_in_cont e5 x5 c)
+  | (cont_sub A) => cont_sub A
+end.
+
+Definition subst_tvar_in_dbind (A5:typ) (X5:typvar) (db5:dbind) : dbind :=
+  match db5 with
+  | dbind_tvar_empty => dbind_tvar_empty 
+  | dbind_stvar_empty => dbind_stvar_empty 
+  | (dbind_typ A) => dbind_typ (subst_tvar_in_typ A5 X5 A)
+end.
+
+Definition subst_tvar_in_work (A_5:typ) (X5:typvar) (w5:work) : work :=
+  match w5 with
+  | (work_infer e c) => work_infer (subst_tvar_in_exp A_5 X5 e) (subst_tvar_in_cont A_5 X5 c)
+  | (work_check e A) => work_check (subst_tvar_in_exp A_5 X5 e) (subst_tvar_in_typ A_5 X5 A)
+  | (work_infabs A c) => work_infabs (subst_tvar_in_typ A_5 X5 A) (subst_tvar_in_cont A_5 X5 c)
+  | (work_infabsunion A1 A2 c) => work_infabsunion (subst_tvar_in_typ A_5 X5 A1) (subst_tvar_in_typ A_5 X5 A2) (subst_tvar_in_cont A_5 X5 c)
+  | (work_infapp A e c) => work_infapp (subst_tvar_in_typ A_5 X5 A) (subst_tvar_in_exp A_5 X5 e) (subst_tvar_in_cont A_5 X5 c)
+  | (work_inftapp A1 A2 c) => work_inftapp (subst_tvar_in_typ A_5 X5 A1) (subst_tvar_in_typ A_5 X5 A2) (subst_tvar_in_cont A_5 X5 c)
+  | (work_sub A1 A2) => work_sub (subst_tvar_in_typ A_5 X5 A1) (subst_tvar_in_typ A_5 X5 A2)
+  | (work_inftappunion A1 A2 B c) => work_inftappunion (subst_tvar_in_typ A_5 X5 A1) (subst_tvar_in_typ A_5 X5 A2) (subst_tvar_in_typ A_5 X5 B) (subst_tvar_in_cont A_5 X5 c)
+  | (work_unioninftapp A1 A2 c) => work_unioninftapp (subst_tvar_in_typ A_5 X5 A1) (subst_tvar_in_typ A_5 X5 A2) (subst_tvar_in_cont A_5 X5 c)
+  | (work_unioninfabs A1 A2 c) => work_unioninfabs (subst_tvar_in_typ A_5 X5 A1) (subst_tvar_in_typ A_5 X5 A2) (subst_tvar_in_cont A_5 X5 c)
+  | (work_apply c A) => work_apply (subst_tvar_in_cont A_5 X5 c) (subst_tvar_in_typ A_5 X5 A)
 end.
 
 Definition subst_var_in_work (e5:exp) (x5:expvar) (w5:work) : work :=
@@ -964,26 +986,12 @@ Definition subst_tvar_in_abind (A_5:typ) (X5:typvar) (ab5:abind) : abind :=
   | (abind_bound A1 B1) => abind_bound (subst_tvar_in_typ A_5 X5 A1) (subst_tvar_in_typ A_5 X5 B1)
 end.
 
-Definition subst_tvar_in_work (A_5:typ) (X5:typvar) (w5:work) : work :=
-  match w5 with
-  | (work_infer e c) => work_infer (subst_tvar_in_exp A_5 X5 e) (subst_tvar_in_cont A_5 X5 c)
-  | (work_check e A) => work_check (subst_tvar_in_exp A_5 X5 e) (subst_tvar_in_typ A_5 X5 A)
-  | (work_infabs A c) => work_infabs (subst_tvar_in_typ A_5 X5 A) (subst_tvar_in_cont A_5 X5 c)
-  | (work_infabsunion A1 A2 c) => work_infabsunion (subst_tvar_in_typ A_5 X5 A1) (subst_tvar_in_typ A_5 X5 A2) (subst_tvar_in_cont A_5 X5 c)
-  | (work_infapp A e c) => work_infapp (subst_tvar_in_typ A_5 X5 A) (subst_tvar_in_exp A_5 X5 e) (subst_tvar_in_cont A_5 X5 c)
-  | (work_inftapp A1 A2 c) => work_inftapp (subst_tvar_in_typ A_5 X5 A1) (subst_tvar_in_typ A_5 X5 A2) (subst_tvar_in_cont A_5 X5 c)
-  | (work_sub A1 A2) => work_sub (subst_tvar_in_typ A_5 X5 A1) (subst_tvar_in_typ A_5 X5 A2)
-  | (work_inftappunion A1 A2 B c) => work_inftappunion (subst_tvar_in_typ A_5 X5 A1) (subst_tvar_in_typ A_5 X5 A2) (subst_tvar_in_typ A_5 X5 B) (subst_tvar_in_cont A_5 X5 c)
-  | (work_unioninftapp A1 A2 c) => work_unioninftapp (subst_tvar_in_typ A_5 X5 A1) (subst_tvar_in_typ A_5 X5 A2) (subst_tvar_in_cont A_5 X5 c)
-  | (work_unioninfabs A1 A2 c) => work_unioninfabs (subst_tvar_in_typ A_5 X5 A1) (subst_tvar_in_typ A_5 X5 A2) (subst_tvar_in_cont A_5 X5 c)
-  | (work_apply c A) => work_apply (subst_tvar_in_cont A_5 X5 c) (subst_tvar_in_typ A_5 X5 A)
-end.
-
-Definition subst_tvar_in_dbind (A5:typ) (X5:typvar) (db5:dbind) : dbind :=
-  match db5 with
-  | dbind_tvar_empty => dbind_tvar_empty 
-  | dbind_stvar_empty => dbind_stvar_empty 
-  | (dbind_typ A) => dbind_typ (subst_tvar_in_typ A5 X5 A)
+Fixpoint subst_tvar_in_dworklist (A5:typ) (X5:typvar) (Ω5:dworklist) {struct Ω5} : dworklist :=
+  match Ω5 with
+  | dworklist_empty => dworklist_empty 
+  | (dworklist_consvar Ω x db) => dworklist_consvar (subst_tvar_in_dworklist A5 X5 Ω) x (subst_tvar_in_dbind A5 X5 db)
+  | (dworklist_constvar Ω X db) => dworklist_constvar (subst_tvar_in_dworklist A5 X5 Ω) X (subst_tvar_in_dbind A5 X5 db)
+  | (dworklist_conswork Ω w) => dworklist_conswork (subst_tvar_in_dworklist A5 X5 Ω) (subst_tvar_in_work A5 X5 w)
 end.
 
 Definition subst_var_in_dvalue (e5:exp) (x5:expvar) (v5:dvalue) : dvalue :=
@@ -1009,13 +1017,6 @@ Fixpoint subst_tvar_in_aworklist (A5:typ) (X5:typvar) (aW_5:aworklist) {struct a
   | (aworklist_conswork aW w) => aworklist_conswork (subst_tvar_in_aworklist A5 X5 aW) (subst_tvar_in_work A5 X5 w)
 end.
 
-Definition subst_tvar_in_dvalue (A5:typ) (X5:typvar) (v5:dvalue) : dvalue :=
-  match v5 with
-  | dvalue_unit => dvalue_unit 
-  | (dvalue_abs e) => dvalue_abs (subst_tvar_in_exp A5 X5 e)
-  | (dvalue_tabs body5) => dvalue_tabs (subst_tvar_in_body A5 X5 body5)
-end.
-
 Fixpoint subst_var_in_aworklist (e5:exp) (x5:expvar) (aW_5:aworklist) {struct aW_5} : aworklist :=
   match aW_5 with
   | aworklist_empty => aworklist_empty 
@@ -1024,12 +1025,11 @@ Fixpoint subst_var_in_aworklist (e5:exp) (x5:expvar) (aW_5:aworklist) {struct aW
   | (aworklist_conswork aW w) => aworklist_conswork (subst_var_in_aworklist e5 x5 aW) (subst_var_in_work e5 x5 w)
 end.
 
-Fixpoint subst_tvar_in_dworklist (A5:typ) (X5:typvar) (Ω5:dworklist) {struct Ω5} : dworklist :=
-  match Ω5 with
-  | dworklist_empty => dworklist_empty 
-  | (dworklist_consvar Ω x db) => dworklist_consvar (subst_tvar_in_dworklist A5 X5 Ω) x (subst_tvar_in_dbind A5 X5 db)
-  | (dworklist_constvar Ω X db) => dworklist_constvar (subst_tvar_in_dworklist A5 X5 Ω) X (subst_tvar_in_dbind A5 X5 db)
-  | (dworklist_conswork Ω w) => dworklist_conswork (subst_tvar_in_dworklist A5 X5 Ω) (subst_tvar_in_work A5 X5 w)
+Definition subst_tvar_in_dvalue (A5:typ) (X5:typvar) (v5:dvalue) : dvalue :=
+  match v5 with
+  | dvalue_unit => dvalue_unit 
+  | (dvalue_abs e) => dvalue_abs (subst_tvar_in_exp A5 X5 e)
+  | (dvalue_tabs body5) => dvalue_tabs (subst_tvar_in_body A5 X5 body5)
 end.
 
 
@@ -1517,6 +1517,29 @@ Inductive a_wf_typ : aenv -> typ -> Prop :=    (* defn a_wf_typ *)
      a_wf_typ aE A2 ->
      a_wf_typ aE (typ_intersection A1 A2).
 
+(* defns J_a_mono_typ *)
+Inductive a_mono_typ : aenv -> typ -> Prop :=    (* defn a_mono_typ *)
+ | a_mono_typ__unit : forall (aE:aenv),
+     a_mono_typ aE typ_unit
+ | a_mono_typ__tvar : forall (aE:aenv) (X:typvar),
+      binds ( X )  ( abind_tvar_empty ) ( aE )  ->
+     a_mono_typ aE (typ_var_f X)
+ | a_mono_typ__etvar : forall (aE:aenv) (X:typvar) (A B:typ),
+      binds ( X )  ( (abind_bound A B) ) ( aE )  ->
+     a_mono_typ aE (typ_var_f X)
+ | a_mono_typ__arrow : forall (aE:aenv) (A1 A2:typ),
+     a_mono_typ aE A1 ->
+     a_mono_typ aE A2 ->
+     a_mono_typ aE (typ_arrow A1 A2)
+ | a_mono_typ__intersection : forall (aE:aenv) (A1 A2:typ),
+     a_mono_typ aE A1 ->
+     a_mono_typ aE A2 ->
+     a_mono_typ aE (typ_intersection A1 A2)
+ | a_mono_typ__union : forall (aE:aenv) (A1 A2:typ),
+     a_mono_typ aE A1 ->
+     a_mono_typ aE A2 ->
+     a_mono_typ aE (typ_union A1 A2).
+
 (* defns J_a_wf_exp *)
 Inductive a_wf_exp : aenv -> exp -> Prop :=    (* defn a_wf_exp *)
  | a_wf_exp__unit : forall (aE:aenv),
@@ -1656,8 +1679,8 @@ Inductive a_wf_wl : aworklist -> Prop :=    (* defn a_wf_wl *)
      a_wf_wl (aworklist_constvar aW X abind_stvar_empty)
  | a_wf_wl__consetvar : forall (aW:aworklist) (X:typvar) (A B:typ),
       ( X   `notin` dom (  ( awl_to_aenv  aW  )  ))  ->
-     a_wf_typ  ( awl_to_aenv  aW  )  A ->
-     a_wf_typ  ( awl_to_aenv  aW  )  B ->
+      ( a_mono_typ  ( awl_to_aenv  aW  )  A ) \/ (  ( A  = typ_bot)  )  ->
+      ( a_mono_typ  ( awl_to_aenv  aW  )  B ) \/ (  ( B  = typ_top)  )  ->
      a_wf_wl aW ->
      a_wf_wl (aworklist_constvar aW X (abind_bound A B))
  | a_wf_wl__conswork : forall (aW:aworklist) (w:work),
@@ -1667,6 +1690,6 @@ Inductive a_wf_wl : aworklist -> Prop :=    (* defn a_wf_wl *)
 
 
 (** infrastructure *)
-#[export] Hint Constructors ds_in neq_abs neq_all neq_intersection neq_union neq_bot d_wf_typ d_wf_exp d_wf_body d_wf_env d_mono_typ d_wf_cont d_wf_work d_wf_wl d_sub a_smono_typ a_evs_in_wl a_wf_typ a_wf_exp a_wf_body a_wf_cont a_wf_work a_wf_wl lc_typ lc_exp lc_body lc_cont lc_dbind lc_work lc_abind lc_dvalue lc_dworklist lc_aworklist : core.
+#[export] Hint Constructors ds_in neq_abs neq_all neq_intersection neq_union neq_bot d_wf_typ d_wf_exp d_wf_body d_wf_env d_mono_typ d_wf_cont d_wf_work d_wf_wl d_sub a_smono_typ a_evs_in_wl a_wf_typ a_mono_typ a_wf_exp a_wf_body a_wf_cont a_wf_work a_wf_wl lc_typ lc_exp lc_body lc_cont lc_dbind lc_work lc_abind lc_dworklist lc_dvalue lc_aworklist : core.
 
 
