proof/iu_system/uni/algo_worklist/prop_soundness.v
@@ -10,26 +10,74 @@ Require Import uni.algo_worklist.transfer.
 Require Import ln_utils.
 
 
+Hint Constructors a_wf_wl : Hdb_a_wl_red_soundness.
+Hint Constructors inst_typ : Hdb_a_wl_red_soundness.
+Hint Constructors inst_cont : Hdb_a_wl_red_soundness.
+Hint Constructors inst_work : Hdb_a_wl_red_soundness.
+Hint Constructors inst_worklist : Hdb_a_wl_red_soundness.
+Hint Constructors wf_ss : Hdb_a_wl_red_soundness.
 Hint Constructors d_wl_del_red : Hdb_a_wl_red_soundness.
+
+
+
+Ltac destruct_a_wf_wl :=
+  repeat
+    match goal with
+    | H : a_wf_wl (aworklist_conswork ?Γ ?w) |- _ => dependent destruction H
+    | H : a_wf_wl (aworklist_consvar ?Γ ?w ?b) |- _ => dependent destruction H
+    | H : a_wf_wl (aworklist_constvar ?Γ ?X ?b) |- _ => dependent destruction H
+    | H : a_wf_work ?Ω ?w |- _ => dependent destruction H
+    | H : a_wf_typ ?E (?Ct ?A1 ?A2) |- _ => dependent destruction H
+    | H : a_wf_exp ?E (?Ce ?b) |- _ => dependent destruction H
+    | H : a_wf_exp ?E (?Ce ?e1 ?e2) |- _ => dependent destruction H
+    end.
+
+
+Ltac _apply_IH_a_wl_red :=
+  let H := fresh "H" in
+    match goal with 
+    | H : (⊢ᵃ ?Γ) -> ?P |- _ => destruct_a_wf_wl; 
+      let H1 := fresh "H" in
+      assert (H1 : ⊢ᵃ Γ) by auto with Hdb_a_wl_red_soundness;
+      apply H in H1
+    end.
+
+Lemma a_wf_wl_wf_ss : forall θ Γ Ω,  
+  ⊢ᵃ Γ -> nil ⫦ Γ ⇝ Ω ⫣ θ -> wf_ss θ.
+Proof.
+Admitted.
 
 
 Theorem d_a_wl_red_soundness: forall Γ,
   ⊢ᵃ Γ -> Γ ⟶ᵃʷ⁎⋅ -> exists Ω, transfer Γ Ω /\ Ω ⟶ᵈ⁎⋅.
 Proof with auto with Hdb_a_wl_red_soundness.
   intros. induction H0; auto; unfold transfer in *.
+  - exists dworklist_empty. intuition...
+    exists nil... 
   - dependent destruction H.
     apply IHa_wl_red in H1.
     destruct H1 as [Ω [Htr Hd_red]].
     admit.
-  - dependent destruction H. 
-    apply IHa_wl_red in H0.
-    destruct H0 as [Ω [Htrans Hd_red]].
+  - _apply_IH_a_wl_red.
+    destruct H2 as [Ω [Htrans Hd_red]].
     destruct Htrans as [θ Htrans].
     exists (dworklist_constvar Ω X dbind_tvar_empty).
-    econstructor. exists ((X, ss_bind__tvar_empty) :: θ).
+    split. exists ((X, ss_bind__tvar_empty) :: θ).
     apply inst_wl__cons_tvar; auto.
     econstructor...
   - admit.
+  - _apply_IH_a_wl_red. 
+    destruct H4 as [Ω [Htrans Hd_red]].
+    destruct Htrans as [θ Htrans].
+    dependent destruction Htrans.
+    dependent destruction H5.
+    admit.
   - admit.
-  -
+  - admit.
+  - _apply_IH_a_wl_red. 
+    destruct H3 as [Ω [Htrans Hd_red]].
+    destruct Htrans as [θ Htrans].
+    exists (dworklist_conswork Ω (work_sub typ_unit typ_unit)).
+    split... exists θ... econstructor; eauto... econstructor. econstructor. admit.
+
 Admitted.
